views: remove need for lenfits

src/lib/data/Kuiper.Matrix.Reprs.Type.fsti
@@ -26,11 +26,17 @@ inline_for_extraction
 class clayout (#rows #cols : erased nat) (l : mlayout rows cols) = {
   [@@@no_method]  m_rows : (x:SZ.t {SZ.v x == reveal rows});
   [@@@no_method]  m_cols : (x:SZ.t {SZ.v x == reveal cols});
-  [@@@no_method]  lenfits : squash (SZ.fits (rows * cols));
   [@@@no_method]  c_to    : (i:SZ.t{i < rows}) -> (j:SZ.t{j < cols}) -> r:SZ.t{SZ.v r == l.bij.ff (SZ.v i, SZ.v j)};
   [@@@no_method]  c_from1 : (idx:SZ.t{idx < rows * cols}) -> r:SZ.t{SZ.v r == fst (l.bij.gg (SZ.v idx))};
   [@@@no_method]  c_from2 : (idx:SZ.t{idx < rows * cols}) -> r:SZ.t{SZ.v r == snd (l.bij.gg (SZ.v idx))};
 }
+
+#push-options "--warn_error -288"
+val clayout_fits (#rows #cols : nat) (#l : mlayout rows cols)
+  (c : clayout l)
+  : Lemma (SZ.fits (mlayout_size l))
+          [SMTPat (has_type c (clayout l))]
+#pop-options
 
 inline_for_extraction
 type crepr_t (r : mrepr) =
