src/lib/data/Kuiper.Matrix.Reprs.Type.fst
@@ -1,0 +1,16 @@
+module Kuiper.Matrix.Reprs.Type
+#lang-pulse
+
+open Kuiper
+open Kuiper.Bijection
+open FStar.Tactics.Typeclasses
+module SZ = FStar.SizeT
+
+#push-options "--warn_error -288"
+let clayout_fits (#rows #cols : nat) (#l : mlayout rows cols)
+  (c : clayout l)
+  : Lemma (SZ.fits (mlayout_size l))
+  = admit()
+    (* I feel this should be provable: c_to is injective and has rows * cols distinct
+    arguments, and returns size_t's (that fit). *)
+#pop-options
